Solved compilation problem in first theorem.

language_formalisation/type_system/type_aux_lemmas.v
@@ -1,9 +1,9 @@
-(* Add LoadPath "C:\Users\Ziga\Documents\Ziga_podatki\PHD\language_formalisation\syntax". *)
-(* Add LoadPath "C:\Users\Ziga\Documents\Ziga_podatki\PHD\language_formalisation\type_system". *)
-(* Add LoadPath "C:\Users\Ziga\Documents\Ziga_podatki\PHD\language_formalisation\substitution". *)
-Add LoadPath "E:\Ziga_Podatki\faks\PHD\language_formalisation\syntax".
-Add LoadPath "E:\Ziga_Podatki\faks\PHD\language_formalisation\type_system".
-Add LoadPath "E:\Ziga_Podatki\faks\PHD\language_formalisation\substitution".
+Add LoadPath "C:\Users\Ziga\Documents\Ziga_podatki\PHD\language_formalisation\syntax".
+Add LoadPath "C:\Users\Ziga\Documents\Ziga_podatki\PHD\language_formalisation\type_system".
+Add LoadPath "C:\Users\Ziga\Documents\Ziga_podatki\PHD\language_formalisation\substitution".
+(* Add LoadPath "E:\Ziga_Podatki\faks\PHD\language_formalisation\syntax". *)
+(* Add LoadPath "E:\Ziga_Podatki\faks\PHD\language_formalisation\type_system". *)
+(* Add LoadPath "E:\Ziga_Podatki\faks\PHD\language_formalisation\substitution". *)
 
 Require Export syntax syntax_lemmas declarational substitution Omega Logic.
 Require Export subs_lemmas wellfounded_lemmas.
@@ -16,8 +16,259 @@ Lemma extend_get_proof Γ A i Ai:
 Proof.
 assert (i + 1 = S i) by omega.
 induction Γ; rewrite H; auto.
-Defined.
+Qed.
 
+Fixpoint v_insert_typesafe v Γ A A_ins i {struct v} :
+  has_vtype Γ v A -> wf_vtype A_ins ->
+  has_vtype (ctx_insert_var Γ A_ins i) (Sub.v_shift v 1 i) A
+with c_insert_typesafe c Γ C A_ins i {struct c} :
+  has_ctype Γ c C -> wf_vtype A_ins ->
+  has_ctype (ctx_insert_var Γ A_ins i) (Sub.c_shift c 1 i) C
+with h_insert_typesafe h Γ Σ D A_ins i {struct h} :
+  has_htype Γ h Σ D -> wf_vtype A_ins ->
+  has_htype (ctx_insert_var Γ A_ins i) (Sub.h_shift h 1 i) Σ D.
+Proof.
+{
+intros orig wfins. apply TypeV.
+{ clear v_insert_typesafe c_insert_typesafe h_insert_typesafe.
+  apply ctx_insert_wf. inv orig. assumption. assumption. }
+{ clear v_insert_typesafe c_insert_typesafe h_insert_typesafe.
+  inv orig. assumption. }
+inv orig. destruct v.
++ clear v_insert_typesafe c_insert_typesafe h_insert_typesafe.
+  inv H1. simpl. destruct (i <=? num) eqn:cmp.
+  - apply TypeVar. rewrite <-get_ctx_insert_changed.
+    assumption. apply leb_complete in cmp. omega.
+  - apply TypeVar. rewrite <-get_ctx_insert_unchanged.
+    assumption. apply leb_iff_conv in cmp. assumption.
++ clear v_insert_typesafe c_insert_typesafe h_insert_typesafe.
+  inv H1. simpl. apply TypeUnit.
++ clear v_insert_typesafe c_insert_typesafe h_insert_typesafe.
+  inv H1. simpl. apply TypeInt.
++ specialize (v_insert_typesafe v) as IHv.
+  clear v_insert_typesafe c_insert_typesafe h_insert_typesafe.
+  inv H1. simpl. apply TypeInl. apply IHv; assumption.
++ specialize (v_insert_typesafe v) as IHv.
+  clear v_insert_typesafe c_insert_typesafe h_insert_typesafe.
+  inv H1. simpl. apply TypeInr. apply IHv; assumption.
++ specialize (v_insert_typesafe v1) as IHv1.
+  specialize (v_insert_typesafe v2) as IHv2.
+  clear v_insert_typesafe c_insert_typesafe h_insert_typesafe.
+  inv H1. simpl. apply TypePair. 
+  - apply IHv1; assumption.
+  - apply IHv2; assumption.
++ specialize (c_insert_typesafe c) as IHc.
+  clear v_insert_typesafe c_insert_typesafe h_insert_typesafe.
+  inv H1. simpl. apply TypeFun. rewrite ctx_insert_extend.
+  apply IHc; assumption.
++ specialize (h_insert_typesafe h) as IHh.
+  specialize (c_insert_typesafe c) as IHc.
+  clear v_insert_typesafe c_insert_typesafe h_insert_typesafe.
+  inv H1. simpl. apply TypeHandler. rewrite ctx_insert_extend. 
+  - apply IHc; assumption. 
+  - apply IHh; assumption.
+}{
+intros orig wfins. apply TypeC.
+{ clear v_insert_typesafe c_insert_typesafe h_insert_typesafe.
+  apply ctx_insert_wf. inv orig. assumption. assumption. }
+{ clear v_insert_typesafe c_insert_typesafe h_insert_typesafe.
+  inv orig. assumption. }
+inv orig. destruct c.
++ specialize (v_insert_typesafe v) as IHv.
+  clear v_insert_typesafe c_insert_typesafe h_insert_typesafe.
+  inv H1. simpl. apply TypeRet. apply IHv; assumption.
++ specialize (v_insert_typesafe v) as IHv.
+  specialize (c_insert_typesafe c) as IHc.
+  clear v_insert_typesafe c_insert_typesafe h_insert_typesafe.
+  inv H1; simpl. eapply TypeΠMatch.
+  apply IHv. exact H7. assumption.
+  rewrite ctx_insert_extend. rewrite ctx_insert_extend.
+  assert (i+1+1=i+2) by omega. rewrite H1. apply IHc; assumption.
++ specialize (v_insert_typesafe v) as IHv.
+  specialize (c_insert_typesafe c1) as IHc1.
+  specialize (c_insert_typesafe c2) as IHc2.
+  clear v_insert_typesafe c_insert_typesafe h_insert_typesafe.
+  inv H1. simpl. eapply TypeΣMatch.
+  - apply IHv. exact H9. assumption.
+  - rewrite ctx_insert_extend. apply IHc1; assumption. 
+  - rewrite ctx_insert_extend. apply IHc2; assumption. 
++ specialize (v_insert_typesafe v) as IHv.
+  specialize (v_insert_typesafe v0) as IHv0.
+  clear v_insert_typesafe c_insert_typesafe h_insert_typesafe.
+  inv H1. simpl. eapply TypeApp.
+  - apply IHv. exact H5. assumption.
+  - apply IHv0; assumption.
++ specialize (v_insert_typesafe v) as IHv.
+  specialize (c_insert_typesafe c) as IHc.
+  clear v_insert_typesafe c_insert_typesafe h_insert_typesafe.
+  inv H1. simpl. eapply TypeOp. exact H8.
+  - apply IHv; assumption.
+  - rewrite ctx_insert_extend. apply IHc; assumption.
++ specialize (c_insert_typesafe c1) as IHc1.
+  specialize (c_insert_typesafe c2) as IHc2.
+  clear v_insert_typesafe c_insert_typesafe h_insert_typesafe.
+  inv H1. simpl. eapply TypeLetRec.
+  - rewrite ctx_insert_extend. rewrite ctx_insert_extend.
+    assert (i+1+1=i+2) by omega. rewrite H1. apply IHc1. exact H8. assumption.
+  - rewrite ctx_insert_extend.  apply IHc2; assumption.
++ specialize (c_insert_typesafe c1) as IHc1.
+  specialize (c_insert_typesafe c2) as IHc2.
+  clear v_insert_typesafe c_insert_typesafe h_insert_typesafe.
+  inv H1. simpl. eapply TypeDoBind.
+  - apply IHc1. exact H7. assumption.
+  - rewrite ctx_insert_extend. apply IHc2; assumption.
++ specialize (v_insert_typesafe v) as IHv.
+  specialize (c_insert_typesafe c) as IHc.
+  clear v_insert_typesafe c_insert_typesafe h_insert_typesafe.
+  inv H1. simpl. eapply TypeHandle.
+  - apply IHv. exact H5. assumption.
+  - apply IHc; assumption.
+}{
+intros orig wfins. apply TypeH.
+{ clear v_insert_typesafe c_insert_typesafe h_insert_typesafe.
+  apply ctx_insert_wf. inv orig. assumption. assumption. }
+{ clear v_insert_typesafe c_insert_typesafe h_insert_typesafe.
+  inv orig. assumption. }
+{ clear v_insert_typesafe c_insert_typesafe h_insert_typesafe.
+  inv orig. assumption. }
+inv orig. destruct h.
++ inv H2. simpl. clear v_insert_typesafe c_insert_typesafe h_insert_typesafe.
+  apply TypeCasesØ.
++ specialize (h_insert_typesafe h) as IHh.
+  specialize (c_insert_typesafe c) as IHc.
+  clear v_insert_typesafe c_insert_typesafe h_insert_typesafe.
+  inv H2. simpl. apply TypeCasesU.
+  - assert (forall h,
+      find_op_case h o = None ->
+      find_op_case (Sub.h_shift h 1 i) o = None).
+    * intros h' orig. induction h'; auto.
+      simpl in *. destruct (o==o0). discriminate.
+      apply IHh'. assumption.
+    * apply H2. assumption.
+  - apply IHh; assumption.
+  - rewrite ctx_insert_extend. rewrite ctx_insert_extend.
+    assert (i+1+1=i+2) by omega. rewrite H2. apply IHc; assumption.
+}
+Qed.
+
+
+
+Proof.
+{
+clear v_insert_typesafe.
+revert A i. induction v.
++ clear c_insert_typesafe h_insert_typesafe.
+  intros. inv H. inv H3. simpl.
+  apply TypeV. apply ctx_insert_wf; assumption. assumption.
+  assert (
+    (if i <=? num then (name, num + 1) else (name, num))
+      = (name, if i <=? num then num + 1 else num) ) 
+  as same by (destruct (i<=?num); reflexivity).
+  rewrite same. simpl. apply TypeVar.
+  simpl. destruct (i<=?num) eqn:cmp.
+  - erewrite <-get_ctx_insert_changed.
+    * assumption.
+    * apply leb_complete in cmp. omega.
+  - erewrite <-get_ctx_insert_unchanged.
+    * assumption.
+    * apply leb_iff_conv in cmp. omega.
++ clear c_insert_typesafe h_insert_typesafe.
+  intros. inv H. inv H3. simpl.
+  apply TypeV. apply ctx_insert_wf; assumption. assumption. apply TypeUnit.
++ clear c_insert_typesafe h_insert_typesafe.
+  intros. inv H. inv H3. simpl.
+  apply TypeV. apply ctx_insert_wf; assumption. assumption. apply TypeInt.
++ clear c_insert_typesafe h_insert_typesafe.
+  intros. inv H. inv H3. simpl.
+  apply TypeV. apply ctx_insert_wf; assumption. assumption.
+  apply TypeInl. apply IHv; assumption.
++ clear c_insert_typesafe h_insert_typesafe.
+  intros. inv H. inv H3. simpl.
+  apply TypeV. apply ctx_insert_wf; assumption. assumption.
+  apply TypeInr. apply IHv; assumption.
++ clear c_insert_typesafe h_insert_typesafe.
+  intros. inv H. inv H3. simpl.
+  apply TypeV. apply ctx_insert_wf; assumption. assumption.
+  apply TypePair. apply IHv1; assumption. apply IHv2; assumption.
++ clear h_insert_typesafe.
+  intros. inv H. inv H3.
+  apply TypeV. apply ctx_insert_wf; assumption. assumption.
+  simpl. apply TypeFun. rewrite ctx_insert_extend.
+  apply c_insert_typesafe; assumption.
++ intros. inv H. inv H3. simpl.
+  apply TypeV. apply ctx_insert_wf; assumption. assumption.
+  simpl. apply TypeHandler. rewrite ctx_insert_extend. apply c_insert_typesafe.
+  clear c_insert_typesafe.
+  assumption. assumption.
+  apply h_insert_typesafe. assumption. assumption.
+}{
+clear c_insert_typesafe h_insert_typesafe.
+revert Γ C i. induction c.
++ intros. inv H. inv H3.
+  apply TypeC. apply ctx_insert_wf; assumption. assumption.
+  simpl. apply TypeRet. apply v_insert_typesafe; assumption.
++ intros. inv H. inv H3.
+  apply TypeC. apply ctx_insert_wf; assumption. assumption.
+  simpl. eapply TypeΠMatch.
+  - apply v_insert_typesafe. exact H8. assumption.
+  - clear v_insert_typesafe. 
+    rewrite ctx_insert_extend. rewrite ctx_insert_extend.
+    assert (i+1+1=i+2) by omega. rewrite H. apply IHc; assumption.
++ intros. inv H. inv H3.
+  apply TypeC. apply ctx_insert_wf; assumption. assumption.
+  simpl. eapply TypeΣMatch.
+  - clear IHc1 IHc2. apply v_insert_typesafe. exact H10. assumption.
+  - clear v_insert_typesafe IHc2. rewrite ctx_insert_extend. apply IHc1; assumption.
+  - clear v_insert_typesafe IHc1. rewrite ctx_insert_extend. apply IHc2; assumption.
++ intros. inv H. inv H3.
+  apply TypeC. apply ctx_insert_wf; assumption. assumption.
+  simpl. eapply TypeApp.
+  - apply v_insert_typesafe. exact H6. assumption.
+  - apply v_insert_typesafe; assumption.
++ intros. inv H. inv H3.
+  apply TypeC. apply ctx_insert_wf; assumption. assumption.
+  simpl. eapply TypeOp.
+  - exact H9.
+  - clear IHc. apply v_insert_typesafe; assumption.
+  - clear v_insert_typesafe. rewrite ctx_insert_extend. apply IHc; assumption.
++ clear v_insert_typesafe. intros. inv H. inv H3.
+  apply TypeC. apply ctx_insert_wf; assumption. assumption.
+  simpl. eapply TypeLetRec.
+  - clear IHc2. rewrite ctx_insert_extend. rewrite ctx_insert_extend.
+    assert (i+1+1=i+2) by omega. rewrite H. apply IHc1. exact H9. assumption.
+  - clear IHc1. rewrite ctx_insert_extend. apply IHc2; assumption.
++ clear v_insert_typesafe. intros. inv H. inv H3.
+  apply TypeC. apply ctx_insert_wf; assumption. assumption.
+  simpl. eapply TypeDoBind.
+  - clear IHc2. apply IHc1. exact H8. assumption.
+  - clear IHc1. rewrite ctx_insert_extend. apply IHc2; assumption.
++ intros. inv H. inv H3.
+  apply TypeC. apply ctx_insert_wf; assumption. assumption.
+  simpl. eapply TypeHandle.
+  - clear IHc. apply v_insert_typesafe. exact H6. assumption.
+  - clear v_insert_typesafe. apply IHc; assumption.
+}{
+clear h_insert_typesafe v_insert_typesafe.
+revert Γ Σ D i. induction h; intros Γ Σ D i orig wf_Ains; simpl; 
+inv orig; inv H0; inv H1; apply TypeH; try (apply ctx_insert_wf; assumption); 
+try apply WfSigØ || apply WfCty || apply WfSigU; try assumption.
++ clear c_insert_typesafe. apply TypeCasesØ.
++ clear c_insert_typesafe. inv H2.
++ clear c_insert_typesafe. inv H2.
++ inv H2. apply TypeCasesU.
+  - clear c_insert_typesafe IHh. 
+    assert (forall h,
+      find_op_case h op = None ->
+      find_op_case (Sub.h_shift h 1 i) op = None).
+    * intros h' orig. induction h'. assumption.
+      simpl in *. destruct (op==o). discriminate. apply IHh'; assumption.
+    * apply H1. assumption.
+  - clear c_insert_typesafe. apply IHh; assumption.
+  - clear IHh. rewrite ctx_insert_extend. rewrite ctx_insert_extend.
+    assert (i+1+1=i+2) by omega. rewrite H1.
+    apply c_insert_typesafe; assumption.
+}
+Qed.
 
 Fixpoint v_insert_typesafe Γ v A A_ins i {struct v} :
   has_vtype Γ v A -> wf_vtype A_ins ->
@@ -31,8 +282,150 @@ with h_insert_typesafe Γ h Σ D A_ins i {struct h} :
 Proof.
 {
 clear v_insert_typesafe.
-revert A i. induction v; intros A i orig wf_Ains; simpl; 
-inv orig; inv H1; apply TypeV; try (assumption || apply ctx_insert_wf; assumption).
+revert A i. induction v.
++ clear c_insert_typesafe h_insert_typesafe.
+  intros. inv H. inv H3. simpl.
+  apply TypeV. apply ctx_insert_wf; assumption. assumption.
+  assert (
+    (if i <=? num then (name, num + 1) else (name, num))
+      = (name, if i <=? num then num + 1 else num) ) 
+  as same by (destruct (i<=?num); reflexivity).
+  rewrite same. simpl. apply TypeVar.
+  simpl. destruct (i<=?num) eqn:cmp.
+  - erewrite <-get_ctx_insert_changed.
+    * assumption.
+    * apply leb_complete in cmp. omega.
+  - erewrite <-get_ctx_insert_unchanged.
+    * assumption.
+    * apply leb_iff_conv in cmp. omega.
++ clear c_insert_typesafe h_insert_typesafe.
+  intros. inv H. inv H3. simpl.
+  apply TypeV. apply ctx_insert_wf; assumption. assumption. apply TypeUnit.
++ clear c_insert_typesafe h_insert_typesafe.
+  intros. inv H. inv H3. simpl.
+  apply TypeV. apply ctx_insert_wf; assumption. assumption. apply TypeInt.
++ clear c_insert_typesafe h_insert_typesafe.
+  intros. inv H. inv H3. simpl.
+  apply TypeV. apply ctx_insert_wf; assumption. assumption.
+  apply TypeInl. apply IHv; assumption.
++ clear c_insert_typesafe h_insert_typesafe.
+  intros. inv H. inv H3. simpl.
+  apply TypeV. apply ctx_insert_wf; assumption. assumption.
+  apply TypeInr. apply IHv; assumption.
++ clear c_insert_typesafe h_insert_typesafe.
+  intros. inv H. inv H3. simpl.
+  apply TypeV. apply ctx_insert_wf; assumption. assumption.
+  apply TypePair. apply IHv1; assumption. apply IHv2; assumption.
++ clear h_insert_typesafe.
+  intros. inv H. inv H3.
+  apply TypeV. apply ctx_insert_wf; assumption. assumption.
+  simpl. apply TypeFun. rewrite ctx_insert_extend.
+  apply c_insert_typesafe; assumption.
++ intros. inv H. inv H3. simpl.
+  apply TypeV. apply ctx_insert_wf; assumption. assumption.
+  simpl. apply TypeHandler. rewrite ctx_insert_extend. apply c_insert_typesafe.
+  clear c_insert_typesafe.
+  assumption. assumption.
+  apply h_insert_typesafe. assumption. assumption.
+}{
+clear c_insert_typesafe h_insert_typesafe.
+revert Γ C i. induction c.
++ intros. inv H. inv H3.
+  apply TypeC. apply ctx_insert_wf; assumption. assumption.
+  simpl. apply TypeRet. apply v_insert_typesafe; assumption.
++ intros. inv H. inv H3.
+  apply TypeC. apply ctx_insert_wf; assumption. assumption.
+  simpl. eapply TypeΠMatch.
+  - apply v_insert_typesafe. exact H8. assumption.
+  - clear v_insert_typesafe. 
+    rewrite ctx_insert_extend. rewrite ctx_insert_extend.
+    assert (i+1+1=i+2) by omega. rewrite H. apply IHc; assumption.
++ intros. inv H. inv H3.
+  apply TypeC. apply ctx_insert_wf; assumption. assumption.
+  simpl. eapply TypeΣMatch.
+  - clear IHc1 IHc2. apply v_insert_typesafe. exact H10. assumption.
+  - clear v_insert_typesafe IHc2. rewrite ctx_insert_extend. apply IHc1; assumption.
+  - clear v_insert_typesafe IHc1. rewrite ctx_insert_extend. apply IHc2; assumption.
++ intros. inv H. inv H3.
+  apply TypeC. apply ctx_insert_wf; assumption. assumption.
+  simpl. eapply TypeApp.
+  - apply v_insert_typesafe. exact H6. assumption.
+  - apply v_insert_typesafe; assumption.
++ intros. inv H. inv H3.
+  apply TypeC. apply ctx_insert_wf; assumption. assumption.
+  simpl. eapply TypeOp.
+  - exact H9.
+  - clear IHc. apply v_insert_typesafe; assumption.
+  - clear v_insert_typesafe. rewrite ctx_insert_extend. apply IHc; assumption.
++ clear v_insert_typesafe. intros. inv H. inv H3.
+  apply TypeC. apply ctx_insert_wf; assumption. assumption.
+  simpl. eapply TypeLetRec.
+  - clear IHc2. rewrite ctx_insert_extend. rewrite ctx_insert_extend.
+    assert (i+1+1=i+2) by omega. rewrite H. apply IHc1. exact H9. assumption.
+  - clear IHc1. rewrite ctx_insert_extend. apply IHc2; assumption.
++ clear v_insert_typesafe. intros. inv H. inv H3.
+  apply TypeC. apply ctx_insert_wf; assumption. assumption.
+  simpl. eapply TypeDoBind.
+  - clear IHc2. apply IHc1. exact H8. assumption.
+  - clear IHc1. rewrite ctx_insert_extend. apply IHc2; assumption.
++ intros. inv H. inv H3.
+  apply TypeC. apply ctx_insert_wf; assumption. assumption.
+  simpl. eapply TypeHandle.
+  - clear IHc. apply v_insert_typesafe. exact H6. assumption.
+  - clear v_insert_typesafe. apply IHc; assumption.
+}{
+clear h_insert_typesafe v_insert_typesafe.
+revert Γ Σ D i. induction h; intros Γ Σ D i orig wf_Ains; simpl; 
+inv orig; inv H0; inv H1; apply TypeH; try (apply ctx_insert_wf; assumption); 
+try apply WfSigØ || apply WfCty || apply WfSigU; try assumption.
++ clear c_insert_typesafe. apply TypeCasesØ.
++ clear c_insert_typesafe. inv H2.
++ clear c_insert_typesafe. inv H2.
++ inv H2. apply TypeCasesU.
+  - clear c_insert_typesafe IHh. 
+    assert (forall h,
+      find_op_case h op = None ->
+      find_op_case (Sub.h_shift h 1 i) op = None).
+    * intros h' orig. induction h'. assumption.
+      simpl in *. destruct (op==o). discriminate. apply IHh'; assumption.
+    * apply H1. assumption.
+  - clear c_insert_typesafe. apply IHh; assumption.
+  - clear IHh. rewrite ctx_insert_extend. rewrite ctx_insert_extend.
+    assert (i+1+1=i+2) by omega. rewrite H1.
+    apply c_insert_typesafe; assumption.
+}
+Qed.
+
+(*
+Fixpoint v_insert_typesafe Γ v A A_ins i {struct v} :
+  has_vtype Γ v A -> wf_vtype A_ins ->
+  has_vtype (ctx_insert_var Γ A_ins i) (Sub.v_shift v 1 i) A
+with c_insert_typesafe Γ c C A_ins i {struct c} :
+  has_ctype Γ c C -> wf_vtype A_ins ->
+  has_ctype (ctx_insert_var Γ A_ins i) (Sub.c_shift c 1 i) C
+with h_insert_typesafe Γ h Σ D A_ins i {struct h} :
+  has_htype Γ h Σ D -> wf_vtype A_ins ->
+  has_htype (ctx_insert_var Γ A_ins i) (Sub.h_shift h 1 i) Σ D.
+Proof.
+{
+clear v_insert_typesafe.
+revert A i. induction v; intros A i orig wf_Ains.
+Focus 7. 
+  clear h_insert_typesafe. inv orig. inv H1. apply TypeV.
+  apply ctx_insert_wf. assumption. assumption.
+  assumption.
+  simpl. apply TypeFun. rewrite ctx_insert_extend. apply c_insert_typesafe.
+  assumption. assumption.
+Focus 7.
+  inv orig. inv H1. apply TypeV.
+  apply ctx_insert_wf. assumption. assumption.
+  assumption.
+  simpl. apply TypeHandler. rewrite ctx_insert_extend. apply c_insert_typesafe.
+  assumption. assumption.
+  apply h_insert_typesafe. assumption. assumption.
+ 
+all: clear c_insert_typesafe h_insert_typesafe.
+all: inv orig; inv H1; apply TypeV; try (assumption || apply ctx_insert_wf; assumption).
 + simpl. assert (
     (if i <=? num then (name, num + 1) else (name, num))
       = (name, if i <=? num then num + 1 else num) ) 
@@ -50,38 +443,37 @@ inv orig; inv H1; apply TypeV; try (assumption || apply ctx_insert_wf; assumptio
 + apply TypeInl. apply IHv; assumption.
 + apply TypeInr. apply IHv; assumption.
 + apply TypePair; try apply IHv1 || apply IHv2; assumption.
-+ apply TypeFun. rewrite ctx_insert_extend. auto.
-+ apply TypeHandler; auto. rewrite ctx_insert_extend. auto.
 }{
-clear c_insert_typesafe.
+clear c_insert_typesafe h_insert_typesafe.
 revert Γ C i. induction c; intros Γ C i orig wfAins; simpl;
 inv orig; inv H1; apply TypeC; try (assumption || apply ctx_insert_wf; assumption).
 + apply TypeRet. apply v_insert_typesafe; assumption.
 + eapply TypeΠMatch.
   - eapply v_insert_typesafe. exact H7. assumption.
   - rewrite ctx_insert_extend. rewrite ctx_insert_extend.
-    assert (i+1+1=i+2) by omega. rewrite H1. auto.
+    assert (i+1+1=i+2) by omega. rewrite H1. apply IHc; assumption.
 + eapply TypeΣMatch.
   - apply v_insert_typesafe. exact H9. assumption.
-  - rewrite ctx_insert_extend. auto.
-  - rewrite ctx_insert_extend. auto.
+  - rewrite ctx_insert_extend. apply IHc1; assumption.
+  - rewrite ctx_insert_extend. apply IHc2; assumption.
 + eapply TypeApp.
   - apply v_insert_typesafe. exact H5. assumption.
-  - auto.
-+ eapply TypeOp. exact H8. auto.
-  rewrite ctx_insert_extend. auto.
+  - apply v_insert_typesafe; assumption.
++ eapply TypeOp. exact H8. 
+  - apply v_insert_typesafe; assumption.
+  - rewrite ctx_insert_extend. apply IHc; assumption.
 + eapply TypeLetRec.
   - rewrite ctx_insert_extend. rewrite ctx_insert_extend.
     assert (i+1+1=i+2) by omega. rewrite H1. apply IHc1. exact H8. assumption.
-  - rewrite ctx_insert_extend. auto.
+  - rewrite ctx_insert_extend. apply IHc2; assumption.
 + eapply TypeDoBind.
   - apply IHc1. exact H7. assumption.
-  - rewrite ctx_insert_extend. auto.
+  - rewrite ctx_insert_extend. apply IHc2; assumption.
 + eapply TypeHandle.
   - apply v_insert_typesafe. exact H5. assumption.
-  - auto.
+  -  apply IHc; assumption.
 }{
-clear h_insert_typesafe.
+clear h_insert_typesafe v_insert_typesafe.
 revert Γ Σ D i. induction h; intros Γ Σ D i orig wf_Ains; simpl; 
 inv orig; inv H0; inv H1; apply TypeH; try (apply ctx_insert_wf; assumption); 
 try apply WfSigØ || apply WfCty || apply WfSigU; try assumption.
@@ -92,13 +484,16 @@ try apply WfSigØ || apply WfCty || apply WfSigU; try assumption.
   - assert (forall h,
       find_op_case h op = None ->
       find_op_case (Sub.h_shift h 1 i) op = None).
-    * intros h' orig. induction h'; auto.
-      simpl in *. destruct (op==o). discriminate. auto.
+    * intros h' orig. induction h'. assumption.
+      simpl in *. destruct (op==o). discriminate. apply IHh'; assumption.
     * apply H1. assumption.
   - rewrite ctx_insert_extend. rewrite ctx_insert_extend.
-    assert (i+1+1=i+2) by omega. rewrite H1. auto.
+    assert (i+1+1=i+2) by omega. rewrite H1.
+    apply c_insert_typesafe; assumption.
 }
-Defined.
+Qed.
+
+
 
 Fixpoint v_shift_typesafe
   (Γ:ctx) (A0:vtype) v A {struct v} :
@@ -121,7 +516,7 @@ rewrite <-H; inv orig.
 apply v_insert_typesafe. apply TypeV; assumption.
 apply c_insert_typesafe. apply TypeC; assumption.
 apply h_insert_typesafe. apply TypeH; assumption.
-Defined.
+Qed.
 
 
 Fixpoint v_negshift_typesafe
@@ -218,7 +613,7 @@ try (apply ctx_remove_wf; assumption); try (apply WfCty; assumption).
     assert (i+1+1=i+2) by omega. rewrite H8.
     apply c_negshift_typesafe; assumption.
 }
-Defined.
+Qed.
 
 
 Fixpoint v_subs_typesafe
@@ -334,7 +729,7 @@ simpl; inv orig; inv H2; apply TypeH; auto.
     - rewrite <-(v_shift_shift 1 1 0).
       apply v_shift_typesafe. apply v_shift_typesafe. assumption.
 }
-Defined.
+Qed.
 
 Lemma h_has_case Γ h Σ D op A_op B_op:
   has_htype Γ h Σ D ->
@@ -348,4 +743,5 @@ inv typed; inv H1; inv H2.
   - injection gets. intros. subst.
     exists v. exists v0. exists c. reflexivity.
   - apply IHh in H14; assumption.
-Defined.
+Qed.
+*)
