language_formalisation/type_system/wellfounded_lemmas.v
@@ -1,9 +1,9 @@
-(* Add LoadPath "C:\Users\Ziga\Documents\Ziga_podatki\PHD\language_formalisation\syntax". *)
-(* Add LoadPath "C:\Users\Ziga\Documents\Ziga_podatki\PHD\language_formalisation\type_system". *)
-(* Add LoadPath "C:\Users\Ziga\Documents\Ziga_podatki\PHD\language_formalisation\substitution". *)
-Add LoadPath "E:\Ziga_Podatki\faks\PHD\language_formalisation\syntax".
-Add LoadPath "E:\Ziga_Podatki\faks\PHD\language_formalisation\type_system".
-Add LoadPath "E:\Ziga_Podatki\faks\PHD\language_formalisation\substitution".
+Add LoadPath "C:\Users\Ziga\Documents\Ziga_podatki\PHD\language_formalisation\syntax".
+Add LoadPath "C:\Users\Ziga\Documents\Ziga_podatki\PHD\language_formalisation\type_system".
+Add LoadPath "C:\Users\Ziga\Documents\Ziga_podatki\PHD\language_formalisation\substitution".
+(* Add LoadPath "E:\Ziga_Podatki\faks\PHD\language_formalisation\syntax". *)
+(* Add LoadPath "E:\Ziga_Podatki\faks\PHD\language_formalisation\type_system". *)
+(* Add LoadPath "E:\Ziga_Podatki\faks\PHD\language_formalisation\substitution". *)
 
 Require Export syntax syntax_lemmas declarational substitution Omega Logic.
 Require Export subs_lemmas.
@@ -18,7 +18,7 @@ revert i A; induction Γ; intros i A orig wfv.
 + induction i; simpl.
   * apply WfCtxU; assumption.
   * inv orig. apply WfCtxU; try apply IHΓ; assumption.
-Defined.
+Qed.
 
 Lemma ctx_remove_wf Γ i:
   wf_ctx Γ -> wf_ctx (ctx_remove_var Γ i).
@@ -28,7 +28,7 @@ revert i; induction Γ; intros i orig.
 + induction i; simpl; inv orig.
   * assumption.
   * apply WfCtxU; try apply IHΓ; assumption.
-Defined.
+Qed.
 
 Lemma get_op_type_wf Σ op A_op B_op:
   wf_sig Σ -> get_op_type Σ op = Some (A_op, B_op) ->
@@ -43,4 +43,4 @@ induction Σ; intros orig gets; constructor.
 + simpl in *. destruct (op == o).
   - injection gets. intros. subst. inv orig. assumption.
   - inv orig. apply IHΣ; assumption.
-Defined.
+Qed.
